src/Utils.v
@@ -1,0 +1,25 @@
+Require Import List.
+Require Import SimpleIO.IOMonad.
+
+Import ListNotations.
+
+Fixpoint fold_io {A B} (f : A -> B -> IO A) (xs : list B) (a : A) :
+  IO A :=
+  match xs with
+  | [] => ret a
+  | x :: xs' => bind (f a x) (fun a' => fold_io f xs' a')
+  end.
+
+Fixpoint existsb_io {A} (f : A -> IO bool) (xs : list A) : IO bool :=
+  match xs with
+  | [] => ret true
+  | x :: xs' =>
+    bind (f x) (fun b => if b then ret true else existsb_io f xs')
+  end.
+
+Fixpoint traverse_io_ {A} (f : A -> IO unit) (xs : list A) :
+  IO unit :=
+  match xs with
+  | [] => ret tt
+  | x :: xs' => bind (f x) (fun _ => traverse_io_ f xs')
+  end.
